lang_implies_cam

CAM/Semantics.v
@@ -1,5 +1,7 @@
 Require Import CAM.Syntax.
 Require Import Lang.Semantics.
+Require Import Lang.ContextProperties.
+Require Import Coq.Relations.Operators_Properties.
 Require Import Coq.Relations.Relation_Operators.
 
 Reserved Notation "k '==>' k'" (at level 40).
@@ -35,6 +37,20 @@ Inductive cam_red {V : Set} : cam_state V -> cam_state V -> Prop :=
 where "k '==>' k'" := (cam_red k k').
 
 Notation "k '==>*' k'" := (clos_refl_trans_1n _ cam_red k k') (at level 40).
+
+Lemma plug_cam_red : 
+  forall (V:Set) (c1:io_ctx V) (c2:oi_ctx V) (e:expr V),
+    ⟨oi_plug c2 e, c1⟩ ==>* ⟨e, add_io_oi c1 c2⟩.
+Proof.
+  intros. generalize dependent c1. induction c2; intro.
+  - simpl. apply rt1n_refl.
+  - simpl. eapply rt1n_trans.
+    + apply cam_red_let.
+    + apply IHc2.
+  - simpl. eapply rt1n_trans.
+    + apply cam_red_handle.
+    + apply IHc2.
+Qed.
 
 Theorem cam_implies_lang : forall (V:Set) (k:cam_state V) (v:value V),
   k ==>* ⟨v, io_ctx_top⟩ ->
@@ -107,6 +123,431 @@ Proof.
       -- apply IH1. reflexivity.
 Qed.
 
+Inductive atomic_expr {V : Set} : expr V -> Prop :=
+  | atomic_add (n1 n2 : nat) :
+      atomic_expr (e_add (v_nat n1) (v_nat n2))
+  | atomic_app (e : expr (inc V)) (v : value V) :
+      atomic_expr (e_app (v_lam e) v)
+  | atomic_do (l : string) (v : value V) :
+      atomic_expr (e_do l v)
+.
+
+Lemma plug_atomic_eq_plug_oi :
+  forall (V:Set) (c1 c:oi_ctx V) (a e:expr V),
+    oi_plug c a = oi_plug c1 e -> atomic_expr a -> 
+    (exists (c2:oi_ctx V), c = add_oi_oi c1 c2).
+Proof.
+  intros. generalize dependent c1. induction c; simpl; intros.
+  - destruct c1.
+    + simpl in H. exists oi_ctx_hole. simpl. reflexivity.
+    + simpl in H. inversion H0.
+      -- subst. discriminate.
+      -- subst. discriminate.
+      -- subst. discriminate.
+    + simpl in H. inversion H0.
+      -- subst. discriminate.
+      -- subst. discriminate.
+      -- subst. discriminate.
+  - destruct c1.
+    + exists (oi_ctx_let c e0). simpl. reflexivity.
+    + simpl in H. injection H as Hplug He0.
+      subst e0. apply IHc in Hplug.
+      destruct Hplug as [c2 Hc2].
+      exists c2. simpl. rewrite <- Hc2. reflexivity.
+    + simpl in H. discriminate.
+  - destruct c1.
+    + exists (oi_ctx_handle c h). simpl. reflexivity.
+    + simpl in H. discriminate.
+    + simpl in H. injection H as Hplug Hh.
+      subst h0. apply IHc in Hplug.
+      destruct Hplug as [c2 Hc2].
+      exists c2. simpl. rewrite <- Hc2. reflexivity.
+Qed.
+
+Lemma plug_atomic_eq_plug_io :
+  forall (V:Set) (c1 c:io_ctx V) (a e:expr V),
+    io_plug c a = io_plug c1 e -> atomic_expr a -> 
+    (exists (c2:oi_ctx V), c = add_io_oi c1 c2).
+Proof.
+  intros.
+  pose proof plug_atomic_eq_plug_oi (V) (io_to_oi c1) (io_to_oi c) a e as H1.
+  rewrite io_plug_bijection in H.
+  rewrite io_plug_bijection in H.
+  apply H1 in H. clear H1.
+  - destruct H as [c2 Hc2].
+    exists c2.
+    apply oi_implies_io in Hc2.
+    rewrite io_bijection_composition in Hc2.
+    rewrite bijection_add_oi_oi in Hc2.
+    apply Hc2.
+  - assumption.
+Qed.
+
+Inductive compound_expr {V : Set} : expr V -> value V -> oi_ctx V -> Prop :=
+  | compound_let (v : value V) (e2 : expr (inc V)) :
+    compound_expr (e_let v e2) v (oi_ctx_let oi_ctx_hole e2)
+  | compound_handle (v : value V) (h : handler V) :
+    compound_expr (e_handle v h) v (oi_ctx_handle oi_ctx_hole h)
+.
+
+Lemma plug_compound_eq_plug_oi :
+  forall (V:Set) (c1 c c_construct:oi_ctx V) (x e:expr V) (v:value V),
+    oi_plug c x = oi_plug c1 e -> compound_expr x v c_construct ->
+    (c1 = add_oi_oi c c_construct /\ e = v) \/
+    (exists (c2:oi_ctx V), c = add_oi_oi c1 c2 /\ e = oi_plug c2 x).
+Proof.
+  intros. generalize dependent c1. induction c; simpl; intros.
+  - inversion H0.
+    + subst. destruct c1.
+      -- right. exists oi_ctx_hole. simpl. split.
+         ++ reflexivity.
+         ++ simpl in H1. symmetry in H1. assumption.
+      -- left. simpl in H1. injection H1 as H2 H3; subst.
+         destruct c1.
+         ++ simpl in H2. auto.
+         ++ simpl in H2. discriminate.
+         ++ simpl in H2. discriminate.
+      -- simpl in H1. discriminate.
+    + subst. destruct c1.
+      -- right. exists oi_ctx_hole. simpl. split.
+         ++ reflexivity.
+         ++ simpl in H1. symmetry in H1. assumption.
+      -- simpl in H1. discriminate.
+      -- left. simpl in H1. injection H1 as H2 H3; subst.
+         destruct c1.
+         ++ simpl in H2. auto.
+         ++ simpl in H2. discriminate.
+         ++ simpl in H2. discriminate.
+  - destruct c1.
+    + simpl in H. right. exists (oi_ctx_let c e0).
+      simpl. split.
+      -- reflexivity.
+      -- symmetry in H. assumption.
+    + simpl in H. injection H as H1 H2; subst.
+      apply IHc in H1. destruct H1 as [[Hc1 He] | [c2 [Hc He]]].
+      -- left. rewrite <- Hc1. rewrite He. split; reflexivity.
+      -- right. exists c2. simpl. rewrite <- Hc. rewrite He.
+         split; reflexivity.
+    + simpl in H. discriminate.
+  - destruct c1.
+    + simpl in H. right. exists (oi_ctx_handle c h).
+      simpl. split.
+      -- reflexivity.
+      -- symmetry in H. assumption.
+    + simpl in H. discriminate.
+    + simpl in H. injection H as H1 H2; subst.
+      apply IHc in H1. destruct H1 as [[Hc1 He] | [c2 [Hc He]]].
+      -- left. rewrite <- Hc1. rewrite He. split; reflexivity.
+      -- right. exists c2. simpl. rewrite <- Hc. rewrite He.
+         split; reflexivity.
+Qed.
+
+Lemma plug_compound_eq_plug_io :
+  forall (V:Set) (c1 c:io_ctx V) (c_construct:oi_ctx V) (x e:expr V) (v:value V),
+    io_plug c x = io_plug c1 e -> compound_expr x v c_construct ->
+    (c1 = add_io_oi c c_construct /\ e = v) \/
+    (exists (c2:oi_ctx V), c = add_io_oi c1 c2 /\ e = oi_plug c2 x).
+Proof.
+  intros.
+  pose proof plug_compound_eq_plug_oi
+    V (io_to_oi c1) (io_to_oi c) c_construct x e v as H1.
+  rewrite io_plug_bijection in H.
+  rewrite io_plug_bijection in H.
+  apply H1 in H; try assumption. clear H1.
+  destruct H as [[Hc1 He] | [c2 [Hc2 He]]].
+  - left. split.
+    + apply oi_implies_io in Hc1.
+      rewrite io_bijection_composition in Hc1.
+      rewrite bijection_add_oi_oi in Hc1.
+      assumption.
+    + assumption.
+  - right. exists c2. split.
+    + apply oi_implies_io in Hc2.
+      rewrite io_bijection_composition in Hc2.
+      rewrite bijection_add_oi_oi in Hc2.
+      assumption.
+    + assumption.
+Qed.
+
+Lemma plug_handle_do_eq_plug_oi :
+  forall (V:Set) (c c1 ch:oi_ctx V) (e:expr V) (h:handler V) (l:string) (v:value V),
+      oi_plug c (e_handle (oi_plug ch (e_do l v)) h) = oi_plug c1 e ->
+      ((exists (c2:oi_ctx V), c = add_oi_oi c1 c2 /\ e = oi_plug c2 (e_handle (oi_plug ch (e_do l v)) h))
+      \/ (exists (ch1 ch2:oi_ctx V), ch = add_oi_oi ch1 ch2 /\ c1 = add_oi_oi c (oi_ctx_handle ch1 h) /\ e = oi_plug ch2 (e_do l v))).
+Proof.
+  intros. generalize dependent c1. induction c; intros.
+  - simpl in H.
+    destruct c1.
+    + simpl. simpl in H. left.
+      exists oi_ctx_hole. split.
+      -- reflexivity.
+      -- simpl. symmetry in H. assumption.
+    + simpl in H. discriminate.
+    + simpl in H. simpl.
+      injection H as H1 H2.
+      subst h0.
+      apply plug_atomic_eq_plug_oi in H1 as Hhc2; (try apply atomic_do).
+      destruct Hhc2 as [hc2 Hch].
+      subst ch. right.
+      exists c1. exists hc2.
+      repeat split.
+      rewrite plug_add_oi_oi in H1.
+      apply oi_plug_injection in H1.
+      symmetry in H1.
+      assumption.
+  - simpl in H. simpl.
+    destruct c1.
+    + left. simpl.
+      exists (oi_ctx_let c e0).
+      repeat split.
+      simpl in H. simpl.
+      symmetry in H. assumption.
+    + simpl in H.
+      injection H as H1 H2.
+      subst e1.
+      apply IHc in H1. clear IHc.
+      destruct H1 as [[c2 [Hc2 He]] | [ch1 [ch2 [Hch [Hc1 He]]]]].
+      -- left. exists c2. simpl.
+         rewrite <- Hc2.
+         repeat split.
+         assumption.
+      -- right. exists ch1. exists ch2.
+         repeat split.
+         ++ assumption.
+         ++ rewrite <- Hc1. reflexivity.
+         ++ assumption.
+    + simpl in H.
+      discriminate.
+  - simpl in H. simpl.
+    destruct c1.
+    + left. simpl.
+      exists (oi_ctx_handle c h0).
+      repeat split.
+      simpl in H. simpl.
+      symmetry in H. assumption.
+    + simpl in H.
+      discriminate.
+    + simpl in H.
+      injection H as H1 H2.
+      subst h0.
+      apply IHc in H1. clear IHc.
+      destruct H1 as [[c2 [Hc2 He]] | [ch1 [ch2 [Hch [Hc1 He]]]]].
+      -- left. exists c2. simpl.
+         rewrite <- Hc2.
+         repeat split.
+         assumption.
+      -- right. exists ch1. exists ch2.
+         repeat split.
+         ++ assumption.
+         ++ rewrite <- Hc1. reflexivity.
+         ++ assumption.
+Qed.
+
+Lemma plug_handle_do_eq_plug_io :
+  forall (V:Set) (c1 c:io_ctx V) (ch:oi_ctx V) (e:expr V) (h:handler V) (l:string) (v:value V),
+      io_plug c (e_handle (oi_plug ch (e_do l v)) h) = io_plug c1 e ->
+      ((exists (c2:oi_ctx V), c = add_io_oi c1 c2 /\ e = oi_plug c2 (e_handle (oi_plug ch (e_do l v)) h))
+      \/ (exists (ch1 ch2:oi_ctx V), ch = add_oi_oi ch1 ch2 /\ c1 = add_io_oi (io_ctx_handle c h) ch1 /\ e = oi_plug ch2 (e_do l v))).
+Proof.
+  intros.
+  pose proof plug_handle_do_eq_plug_oi
+    V (io_to_oi c) (io_to_oi c1) ch e h l v as H1.
+  rewrite io_plug_bijection in H.
+  rewrite io_plug_bijection in H.
+  apply H1 in H. clear H1.
+  destruct H as [[c2 [Hc2 He]] | [ch1 [ch2 [Hch [Hc1 He]]]]].
+  - left. exists c2.
+    apply oi_implies_io in Hc2.
+    rewrite io_bijection_composition in Hc2.
+    rewrite bijection_add_oi_oi in Hc2.
+    split.
+    + assumption.
+    + assumption.
+  - right. exists ch1. exists ch2.
+    repeat split.
+    + assumption.
+    + apply oi_implies_io in Hc1.
+      rewrite io_bijection_composition in Hc1.
+      rewrite bijection_add_oi_oi in Hc1.
+      simpl in Hc1. assumption.
+    + assumption.
+Qed.
+
+Lemma de_morgan2 : forall (P Q : Prop), ~(P \/ Q) -> ~P /\ ~Q.
+Proof.
+  intros P Q H. split.
+  - intro HP. apply H. left. assumption.
+  - intro HQ. apply H. right. assumption.
+Qed.
+
+Lemma add_io_oi_op_cam_red_io :
+  forall (V:Set) (c1 c2:io_ctx V) (ch:oi_ctx V) (l:string) (v:value V),
+    ~IoCtxHandlesOp c2 l ->
+    ⟨add_io_io c1 c2, ch, l, v⟩ ==>* ⟨c1, add_io_oi2 c2 ch, l, v⟩.
+Proof.
+  intros. generalize dependent ch.
+  induction c2; intro.
+  - simpl. apply rt1n_refl.
+  - simpl. eapply rt1n_trans.
+    + apply cam_red_op_let.
+    + apply IHc2.
+      simpl in H. assumption.
+  - simpl. simpl in H.
+    apply de_morgan2 in H as [H1 H2].
+    eapply rt1n_trans.
+    + apply cam_red_op_handle1. assumption.
+    + apply IHc2. assumption.
+Qed.
+
+Lemma add_io_oi_op_cam_red :
+  forall (V:Set) (c1:io_ctx V) (c2 ch:oi_ctx V) (l:string) (v:value V),
+    ~OiCtxHandlesOp c2 l ->
+    ⟨add_io_oi c1 c2, ch, l, v⟩ ==>* ⟨c1, add_oi_oi c2 ch, l, v⟩.
+Proof.
+  intros.
+  pose proof add_io_oi_op_cam_red_io V c1 (oi_to_io c2) ch l v.
+  apply not_oi_ctx_handles_op_bijection in H.
+  apply H0 in H. clear H0.
+  rewrite add_io_io_eq_add_io_oi in H.
+  rewrite add_io_oi2_eq_add_oi_oi in H.
+  apply H.
+Qed.
+
+Theorem lang_implies_cam : forall (V:Set) (e1:expr V) (v:value V),
+  e1 -->* v -> forall (c:io_ctx V) (e:expr V), e1 = io_plug c e -> ⟨e, c⟩ ==>* ⟨v, io_ctx_top⟩.
+Proof.
+  intros V e1 v Hmulti.
+  remember (e_ret v) as e2.
+  induction Hmulti; intros; subst.
+  - assert (Hplug_eq_v: io_plug c e = v -> c = io_ctx_top /\ e = v).
+    { generalize dependent e. induction c; intro.
+      + simpl. auto.
+      + simpl. intro H. apply IHc in H as [_ H2].
+        -- discriminate H2.
+        -- auto.
+      + simpl. intro H. apply IHc in H as [_ H2].
+        -- discriminate H2. 
+        -- auto.
+    }
+    symmetry in H.
+    apply Hplug_eq_v in H as [Hc He]. subst.
+    simpl. apply rt1n_refl.
+  - apply red_decomposition in H as [c' [r1 [r2 [Hc' [Hy Hr]]]]].
+    subst y.
+    inversion Hr; subst.
+    + symmetry in Hc'.
+      apply plug_atomic_eq_plug_io in Hc' as Hc2; try (apply atomic_add).
+      destruct Hc2 as [c2 Hc2]. subst c'.
+      rewrite plug_add_io_oi in Hc'.
+      apply io_plug_injection in Hc'.
+      rewrite <- Hc'.
+      apply clos_rt_rt1n.
+      eapply rt_trans; (apply clos_rt1n_rt).
+      -- apply plug_cam_red.
+      -- eapply rt1n_trans.
+         ++ apply cam_red_add.
+         ++ apply IHHmulti; reflexivity.
+    + symmetry in Hc'.
+      apply plug_atomic_eq_plug_io in Hc' as Hc2; try (apply atomic_app).
+      destruct Hc2 as [c2 Hc2]. subst c'.
+      rewrite plug_add_io_oi in Hc'.
+      apply io_plug_injection in Hc'.
+      rewrite <- Hc'.
+      apply clos_rt_rt1n.
+      eapply rt_trans; (apply clos_rt1n_rt).
+      -- apply plug_cam_red.
+      -- eapply rt1n_trans.
+         ++ apply cam_red_app.
+         ++ apply IHHmulti; reflexivity.
+    + symmetry in Hc'.
+      apply plug_compound_eq_plug_io with
+        (c_construct := oi_ctx_let oi_ctx_hole e0) (v := v0) in Hc' as Hc_shape;
+      try apply compound_let.
+      destruct Hc_shape as [[Hc He] | [c2 [Hc2 He]]].
+      -- subst. simpl.
+         eapply rt1n_trans.
+         ++ apply cam_red_ret_let.
+         ++ apply IHHmulti; reflexivity.
+      -- subst. 
+         apply clos_rt_rt1n.
+         eapply rt_trans; (apply clos_rt1n_rt).
+         ++ apply plug_cam_red.
+         ++ eapply rt1n_trans.
+            ** apply cam_red_let.
+            ** eapply rt1n_trans.
+               *** apply cam_red_ret_let.
+               *** apply IHHmulti; reflexivity.
+    + symmetry in Hc'.
+      apply plug_compound_eq_plug_io with
+        (c_construct := oi_ctx_handle oi_ctx_hole h) (v := v0) in Hc' as Hc_shape;
+      try apply compound_handle.
+      destruct Hc_shape as [[Hc He] | [c2 [Hc2 He]]].
+      -- subst. simpl.
+         eapply rt1n_trans.
+         ++ apply cam_red_ret_handle.
+         ++ apply IHHmulti; reflexivity.
+      -- subst. 
+         apply clos_rt_rt1n.
+         eapply rt_trans; (apply clos_rt1n_rt).
+         ++ apply plug_cam_red.
+         ++ eapply rt1n_trans.
+            ** apply cam_red_handle.
+            ** eapply rt1n_trans.
+               *** apply cam_red_ret_handle.
+               *** apply IHHmulti; reflexivity.
+    + symmetry in Hc'.
+      apply plug_handle_do_eq_plug_io in Hc' as Hc_shape.
+      destruct Hc_shape as [[c2 [Hc2 He]] | [ch1 [ch2 [Hhc [Hc He]]]]].
+      -- subst.
+         apply clos_rt_rt1n.
+         eapply rt_trans; (apply clos_rt1n_rt).
+         ++ apply plug_cam_red.
+         ++ eapply rt1n_trans.
+            ** apply cam_red_handle.
+            ** apply clos_rt_rt1n.
+               eapply rt_trans; (apply clos_rt1n_rt).
+               *** apply plug_cam_red.
+               *** eapply rt1n_trans.
+                   **** apply cam_red_do.
+                   **** apply clos_rt_rt1n.
+                        eapply rt_trans; (apply clos_rt1n_rt).
+                        ***** apply add_io_oi_op_cam_red.
+                              assumption.
+                        ***** rewrite add_oi_oi_hole_r.
+                              eapply rt1n_trans.
+                              ****** eapply cam_red_op_handle2.
+                                     apply He_op.
+                              ****** apply IHHmulti; reflexivity.
+      -- subst.
+         apply clos_rt_rt1n.
+         eapply rt_trans; (apply clos_rt1n_rt).
+         ++ apply plug_cam_red.
+         ++ eapply rt1n_trans.
+            ** apply cam_red_do.
+            ** apply not_oi_ctx_handles_op_add in Hctx as [Hch1 Hch2].
+               apply clos_rt_rt1n.
+               eapply rt_trans; (apply clos_rt1n_rt).
+               *** apply add_io_oi_op_cam_red.
+                   assumption.
+               *** apply clos_rt_rt1n.
+                   eapply rt_trans; (apply clos_rt1n_rt).
+                   **** apply add_io_oi_op_cam_red.
+                        assumption.
+                   **** rewrite add_oi_oi_hole_r.
+                        eapply rt1n_trans.
+                        ***** apply cam_red_op_handle2.
+                              apply He_op.
+                        ***** apply IHHmulti; reflexivity.
+Qed.
+
 Theorem lang_equiv_cam : forall (V:Set) (e:expr V) (v:value V),
   e -->* v <-> ⟨e, io_ctx_top⟩ ==>* ⟨v, io_ctx_top⟩.
-Admitted.
+Proof.
+  intros V e v. split; intro.
+  - apply lang_implies_cam with (e1 := e).
+    + assumption.
+    + simpl. reflexivity.
+  - apply cam_implies_lang in H as [H1 _].
+    apply H1 with (c := io_ctx_top).
+    reflexivity.
+Qed.
