Lang/Semantics.v
@@ -1,4 +1,5 @@
 Require Import Lang.Syntax.
+Require Import Lang.ContextProperties.
 Require Import Coq.Relations.Relation_Operators.
 
 Reserved Notation "e '-->' e'" (at level 40).
@@ -36,4 +37,56 @@ Definition nat_refl :
   (e_ret (@v_nat Empty_set 42)) -->* (e_ret (@v_nat Empty_set 42)).
 Proof.
   apply rt1n_refl.
+Qed.
+
+Reserved Notation "e '~~>' e'" (at level 40).
+
+Inductive contraction {V : Set} : expr V -> expr V -> Prop :=
+  | contraction_add (n1 n2 : nat) :
+      (e_add (v_nat n1) (v_nat n2)) ~~> (e_ret (v_nat (n1 + n2)))
+  | contraction_app (e : expr (inc V)) (v : value V) :
+      (e_app (v_lam e) v) ~~> (esubst e v)
+  | contraction_let (v : value V) (e : expr (inc V)) :
+      (e_let (e_ret v) e) ~~> (esubst e v)
+  | contraction_handle_ret (v : value V) (h : handler V) :
+      (e_handle (e_ret v) h) ~~> (esubst (ret_clause h) v)
+  | contraction_handle_do
+      (h : handler V)
+      (l : string)
+      (v : value V)
+      (ctx : oi_ctx V)
+      (e_op : expr (inc (inc V)))
+      (He_op : HandlesOp h l e_op)
+      (Hctx : ~OiCtxHandlesOp ctx l) :
+      (e_handle (oi_plug ctx (e_do l v)) h) ~~>
+      (esubst (esubst e_op (vshift v))
+              (v_lam (oi_plug (oi_shift ctx) (e_ret (v_var VZ)))))
+where "e '~~>' e'" := (contraction e e').
+
+Theorem red_decomposition : forall (V:Set) (e1 e2:expr V),
+  e1 --> e2 ->
+  (exists (c:io_ctx V) (r1 r2:expr V),
+  e1 = io_plug c r1 /\ 
+  e2 = io_plug c r2 /\ 
+  r1 ~~> r2).
+Proof.
+  intros. induction H.
+  - exists io_ctx_top. exists (e_add (v_nat n1) (v_nat n2)). exists (v_nat (n1 + n2)).
+    repeat split; auto. apply contraction_add.
+  - exists io_ctx_top. exists (e_app (v_lam e) v). exists (esubst e v).
+    repeat split; auto. apply contraction_app.
+  - exists io_ctx_top. exists (e_let (e_ret v) e). exists (esubst e v).
+    repeat split; auto. apply contraction_let.
+  - exists  io_ctx_top. exists (e_handle (e_ret v) h). exists (esubst (ret_clause h) v).
+    repeat split; auto. apply contraction_handle_ret.
+  - exists io_ctx_top. exists (e_handle (oi_plug ctx (e_do l v)) h).
+    exists (esubst (esubst e_op (vshift v))
+                   (v_lam (oi_plug (oi_shift ctx) (e_ret (v_var VZ))))).
+    repeat split; auto. apply contraction_handle_do; auto.
+  - destruct IHred as [c' [r1 [r2 [He1 [He2 Hr]]]]].
+    exists (add_io_io c c'). exists r1. exists r2.
+    repeat split; subst.
+    + rewrite plug_add_io_io. reflexivity.
+    + rewrite plug_add_io_io. reflexivity.
+    + apply Hr.
 Qed.
